src/high/generational_resources.v
@@ -1,52 +1,585 @@
-(* The generational resources used by HighSpirea.
- *
- * The following resources are all [ghost_map loc V], and a crash
- * will only shrink the domain of the map, but never changes the value, and thus
- * share (most of) nextgen definition.
- * - the knowledge of protocols
- * - the knowledge of preorder
- * - the knowledge of bumper
- * - the knowledge of atomic and non-atomic locations
- * The following resources were maintained by highSpirea, but it's now maintained
- * in baseSpirea already and we only need to import the definitions:
- * - the offsets for each location
- * - the full physical history including messages from previous generation
- * The following resources require their own nextgen construction:
- * - the view for every non-atomic location (since they are not shared, there is always
- *   a single view one will access)
- * - the abstract history
- *)
+(*** HighSpirea Generational Resources. *)
+From iris.proofmode Require Import proofmode.
+From iris.algebra Require Import gset.
+From iris.bi.lib Require Import fractional.
+From iris_named_props Require Import named_props.
 
-From self Require Import extra.
+From self Require Import extra encode_relation.
 From self.lang Require Import lang.
 
-From self.base Require Export generational_resources.
-From self.nextgen Require Import gen_ing.
-From self.high.resources Require Export
+From self.base Require Export generational_resources if_rec.
+From self.nextgen Require Import gen_ing nextgen_promises.
+From self.high.resources Require Import
   gen_ghost_map gen_ghost_map_map gen_alocs gen_predicates auth_map_map.
-
+From self.high.lib Require Export bumpers abstract_state.
 From self.algebra Require Import view.
 
+(** Typeclasses for highSpirea logic. *)
+Class nvmHighGpreS Σ Ω `{!nvmBaseGS Σ Ω} := {
+  nvmHighGpreS_predicates :: predicatesGpreS Σ Ω;
+  nvmHighGpreS_bumpers :: ghost_mapGpreS loc (positive → option positive) Σ Ω;
+  nvmHighGpreS_abs_histories :: ghost_map_mapGpreS loc time positive Σ Ω;
+  nvmHighGpreS_phys_histories :: auth_map_mapR_inG (leibnizO message) Σ Ω;
+  nvmHighGpreS_na_views :: ghost_mapGpreS loc view Σ Ω;
+  nvmHighGpreS_orders :: ghost_mapGpreS loc (relation2 positive) Σ Ω;
+  nvmHighGpre_locs :: gen_alocsR_inG Σ Ω;
+}.
+
 Class nvmHighGS Σ Ω `{!nvmBaseGS Σ Ω} := NvmHighG {
-  nvm_predicatesG :: (genInDepsG Σ Ω (predicatesR (Σ := Σ)) [#crashed_atR]);
+  #[local] nvmHighGS_inG :: nvmHighGpreS Σ Ω;
   full_predicates_name : gname;
   read_predicates_name : gname;
   pers_predicates_name : gname;
-  abs_historiesG :: ghost_map_mapGpreS loc time positive Σ Ω;
   abs_history_name : gname;
   (* resharing [phy_history] for atomic locations *)
-  phy_historiesG :: auth_map_mapR_inG (leibnizO message) Σ Ω;
   phy_history_name : gname;
-  non_atomic_views :: ghost_mapGpreS loc view Σ Ω;
   non_atomic_views_gname : gname;
-  crashed_in_inG :: ghost_mapGpreS loc positive Σ Ω;
-  crashed_in_name : gname;
-  preordersG :: ghost_mapGpreS loc (relation2 positive) Σ Ω;
   preorders_name : gname;
-  locsG :: gen_alocsR_inG Σ Ω;
   exclusive_locs_name : gname;
   shared_locs_name : gname;
   new_locs_name : gname;
-  nvm_bumpersG :: ghost_mapGpreS loc (positive → option positive) Σ Ω;
   bumpers_name : gname;
 }.
+
+(** we proceed to define assertions that needs to know the [gen_inG] typeclass instances. *)
+Section location_sets.
+  Context `{nvmHighGS}.
+  Implicit Types (locs : gset loc) (ℓ : loc).
+
+  Definition is_at_loc ℓ : iProp Σ :=
+    gen_alocs_frag shared_locs_name {[ ℓ ]}.
+  Definition is_na_loc ℓ : iProp Σ :=
+    gen_alocs_frag exclusive_locs_name {[ ℓ ]}.
+  
+  Lemma location_sets_singleton_included {γ} locs ℓ :
+    gen_alocs_auth γ locs -∗ gen_alocs_frag γ {[ ℓ ]} -∗ ⌜ ℓ ∈ locs ⌝.
+  Proof.
+    iNamed 1. iDestruct 1 as "(own_frag & _)".
+    iDestruct (gen_own_valid_2 with "own_auth own_frag")
+      as %[V%gset_included _]%auth_both_valid_discrete.
+    rewrite elem_of_subseteq_singleton.
+    done.
+  Qed.
+
+  Lemma location_sets_lookup γ locs ℓ :
+    ℓ ∈ locs → gen_alocs_frag γ locs -∗ gen_alocs_frag γ {[ ℓ ]}.
+  Proof.
+    intros.
+    iNamed 1.
+    iPoseProof (gen_own_mono _ _ (◯ {[ ℓ ]}) with "own_frag") as "own_frag".
+    { apply auth_frag_mono. set_solver. }
+    iFrame "∗#".
+  Qed.
+End location_sets.
+
+(* We need a different [offset], that allows us to insert [0] at new locations. *)
+Section offset_loc.
+  Context `{nvmHighGS}.
+
+  Definition offset_auth (offsets: gmap loc nat): iProp Σ :=
+    ∃ (OCV: view),
+      "#crashed" ∷ crashed_at_offset OCV ∗
+      "newLocs" ∷ gen_alocs_auth new_locs_name (dom offsets) ∗
+      "%HLookup" ∷ ⌜ ∀ (ℓ: loc), ℓ ∈ dom offsets → offsets !! ℓ = Some (OCV !!0 ℓ) ⌝.
+
+  Definition offset_loc ℓ (t: nat): iProp Σ :=
+    ∃ OCV, crashed_at_offset OCV ∗
+           gen_alocs_frag new_locs_name {[ ℓ ]} ∗ ⌜ OCV !!0 ℓ = t ⌝.
+
+  Lemma offset_loc_agree ℓ t1 t2 :
+    offset_loc ℓ t1 -∗
+    offset_loc ℓ t2 -∗
+    ⌜ t1 = t2 ⌝.
+  Proof.
+    rewrite /offset_loc.
+    iIntros "(%OCV & crash & new_locs_frag & %look)".
+    iIntros "(%OCV' & crash' & new_locs_frag' & %look')".
+    iDestruct (crashed_at_offset_agree with "[$] [$]") as "->".
+    iPureIntro.
+    congruence.
+  Qed.
+
+  Lemma offset_loc_offset_auth_agree ℓ t offsets :
+    offset_loc ℓ t -∗
+    offset_auth offsets -∗
+    ⌜ offsets !! ℓ = Some t ⌝.
+  Proof.
+    iIntros "(%OCV & crash & new_locs_frag & %look)". iNamed 1.
+    iDestruct (crashed_at_offset_agree with "crash crashed") as "<-".
+    iDestruct (location_sets_singleton_included with "[$] [$]") as "%Hdom".
+    iPureIntro.
+    specialize (HLookup ℓ Hdom).
+    rewrite look /lookup_zero in HLookup.
+    done.
+  Qed.
+
+  Lemma offset_loc_crashed_at_offset_agree ℓ t OCV:
+    offset_loc ℓ t -∗
+    crashed_at_offset OCV -∗
+    ⌜ OCV !!0 ℓ = t ⌝.
+  Proof.
+    iIntros "(% & ? & _ & %) ?".
+    iDestruct (crashed_at_offset_agree with "[$] [$]") as %->.
+    done.
+  Qed.
+  
+  Lemma offset_auth_insert OCV offsets ℓ:
+    ℓ ∉ dom OCV →
+    ℓ ∉ dom offsets →
+    crashed_at_offset OCV -∗
+    offset_auth offsets ==∗
+    offset_auth (<[ ℓ := 0 ]> offsets) ∗ offset_loc ℓ 0.
+  Proof.
+    iIntros (HOCVdom Hoffsetsdom) "crashed'". iNamed 1.
+    iDestruct (crashed_at_offset_agree with "crashed crashed'") as %->.
+    iMod (gen_alocs_update (dom offsets) ℓ with "newLocs") as "[newLocs frag]".
+    iModIntro.
+    iSplitL "newLocs".
+    - iExists _.
+      rewrite dom_insert_L.
+      replace ({[ℓ]} ∪ dom offsets) with (dom offsets ∪ {[ℓ]}); last by set_solver.
+      iFrame "∗#".
+      iPureIntro.
+      intros ℓ'.
+      destruct (decide (ℓ = ℓ')) as [ <- | ].
+      * rewrite lookup_insert_eq lookup_zero_None_zero //.
+        by apply not_elem_of_dom.
+      * rewrite lookup_insert_ne //.
+        intros.
+        apply HLookup.
+        set_solver.
+    - iFrame.
+      rewrite lookup_zero_None_zero //.
+      by apply not_elem_of_dom.
+  Qed.
+
+  #[global] Instance offset_loc_into_nextgen ℓ t:
+    IntoNextgen
+    (offset_loc ℓ t)
+    (if_rec ℓ (∃ tC, offset_loc ℓ tC ∗ ∀ OV OCV, crashed_at_both OV OCV -∗ ⌜ OV !!0 ℓ = t ⌝ ∗ ⌜ OCV !! ℓ = Some (MaxNat tC) ⌝)).
+  Proof.
+    rewrite /IntoNextgen.
+    iDestruct 1 as (OCV) "(offset & newLocs & %)".
+    iAssert (rely new_locs_name [#crashed_at_name] gen_alocs_rel (λ _, true))%I as "#rely".
+    { by iNamed "newLocs". }
+    iModIntro.
+    iDestruct "offset" as (OV) "(%trans & picked & offset)".
+    iDestruct "rely" as "(_ & % & %trans' & %promise & _ & picked')".
+    iPickedInAgree "picked' picked".
+    destruct promise as [(OCV' & -> & _) _].
+    simpl.
+    iIntros (OCV'' HOCVLook) "#crashed #persisted".
+    iSpecialize ("newLocs" with "crashed").
+    iExists _.
+    rewrite /offset_loc.
+    simpl.
+    iDestruct "crashed" as (OV') "crashed".
+    iDestruct (crashed_at_both_agree with "crashed offset") as %[ -> -> ].
+    iSplit.
+    - iExists OCV'.
+      iSplit; first by iExists _.
+      iSplit; last done.
+      assert (ℓ ∈ dom OCV') by (by apply elem_of_dom).
+      iEval (replace ({[ℓ]}) with ({[ℓ]} ∩ dom OCV') by set_solver).
+      done.
+    - iIntros (??) "crashed'".
+      iDestruct (crashed_at_both_agree with "crashed crashed'") as %[ <- <- ].
+      simplify_eq.
+      iSplit; first done.
+      iPureIntro.
+      rewrite /lookup_zero.
+      destruct HOCVLook as [[?] HOCVLook].
+      rewrite ?HOCVLook //.
+  Qed.
+
+  Lemma offset_auth_picked_out (OCV': view) offsets:
+    picked_out crashed_at_name (crashed_at_trans (OCV')) -∗
+    offset_auth offsets -∗
+    ⚡==> offset_auth $ max_nat_car <$> restrict (dom offsets) OCV'.
+  Proof.
+    iIntros "#picked". iNamed 1. iModIntro.
+    iDestruct ("crashed") as (OV' t) "[picked'' crashed]".
+    iPickedInAgree "picked picked''".
+    iAssert (crashed_at_offset OCV')%I as "OCV'".
+    { by iExists _. }
+    iSpecialize ("newLocs" with "OCV'").
+    iExists OCV'.
+    iSplit; first done.
+    iSplitL "newLocs".
+    { rewrite dom_fmap_L restrict_dom_L //. }
+    iPureIntro.
+    intros ℓ look. rewrite lookup_fmap.
+    rewrite dom_fmap_L restrict_dom_L in look.
+    rewrite restrict_lookup_elem_of; last set_solver.
+    rewrite /lookup_zero.
+    assert (ℓ ∈ dom OCV') as [? ->]%elem_of_dom by set_solver.
+    done.
+  Qed.
+
+End offset_loc.
+
+Opaque offset_auth offset_loc.
+
+Section preorders.
+  Context `{nvmHighGS}.
+  Implicit Type (preorders : gmap loc (relation2 positive)).
+  Context `{Countable ST}.
+
+  Definition own_all_preorders γ preorders :=
+    ghost_map_auth γ drop_OCV (DfracOwn 1) preorders.
+
+  Definition know_preorder_loc ℓ (preorder : relation2 ST) : iProp Σ :=
+    ℓ ↪[preorders_name, drop_OCV]□ encode_relation preorder.
+
+  Definition lastgen_know_preorder_loc ℓ (preorder : relation2 ST) : iProp Σ :=
+    lastgen_ghost_map_elem preorders_name ℓ DfracDiscarded (encode_relation preorder).
+  
+  Lemma orders_lookup ℓ order1 order2 (orders : gmap loc (relation2 positive)) :
+    orders !! ℓ = Some order1 →
+    own_all_preorders preorders_name orders -∗
+    know_preorder_loc ℓ order2 -∗
+    ⌜order1 = encode_relation order2⌝.
+  Proof.
+    iIntros (look) "auth frag".
+    iDestruct (ghost_map_lookup with "auth frag") as "%".
+    iPureIntro. congruence.
+  Qed.
+End preorders.
+
+Opaque own_all_preorders know_preorder_loc.
+
+Section own_bumpers.
+  Context `{nvmHighGS} `{AbstractState ST}.
+  
+  Definition own_all_bumpers γ (encoded_bumpers: gmap loc (positive → option positive)): iProp Σ :=
+    ghost_map_auth γ drop_OCV (DfracOwn 1) encoded_bumpers.
+  
+  Definition know_bumper ℓ (bumper : ST → ST) : iProp Σ :=
+    let encodedBumper := encode_bumper bumper in
+    ⌜ ∀ s1 s2, s1 ⊑ s2 → bumper s1 ⊑ bumper s2 ⌝ ∗
+    ℓ ↪[bumpers_name, drop_OCV]□ encodedBumper.
+
+  Definition lastgen_know_bumper (ℓ : loc) (bumper : ST → ST) : iProp Σ :=
+    let encodedBumper := encode_bumper bumper
+    in ⌜∀ s1 s2, s1 ⊑ s2 → bumper s1 ⊑ bumper s2⌝ ∗
+                 lastgen_ghost_map_elem bumpers_name ℓ DfracDiscarded encodedBumper.
+  
+  Lemma own_all_bumpers_persist γ encoded_bumpers :
+    own_all_bumpers γ encoded_bumpers ==∗
+    ghost_map_auth γ drop_OCV DfracDiscarded encoded_bumpers.
+  Proof. by iApply ghost_map_auth_persist. Qed.
+
+  Lemma own_all_bumpers_insert (bumpers : gmap loc _) ℓ (bumper : ST → ST)
+        `{!Proper ((⊑@{ST}) ==> (⊑))%signature bumper} :
+    bumpers !! ℓ = None →
+    own_all_bumpers bumpers_name bumpers ==∗
+    own_all_bumpers bumpers_name (<[ℓ := encode_bumper bumper]>bumpers) ∗ know_bumper ℓ bumper.
+  Proof.
+    rewrite /own_all_bumpers. iIntros (look) "auth".
+    iMod (ghost_map_insert_persist with "auth") as "[$ #bumper]"; first done.
+    iFrame "bumper".
+    done.
+  Qed.
+
+  Lemma bumpers_lookup ℓ encoded_bumpers bumper :
+    own_all_bumpers bumpers_name encoded_bumpers -∗
+    know_bumper ℓ bumper -∗
+    ⌜ encoded_bumpers !! ℓ = Some (encode_bumper bumper) ⌝.
+  Proof.
+    iIntros "A [mono F]".
+    iDestruct (ghost_map_lookup with "A F") as "$".
+  Qed.
+End own_bumpers.
+
+Section NAView.
+  Context `{nvmHighGS}.
+
+  Definition know_na_view ℓ q (SV : view) : iProp Σ :=
+    ℓ ↪[non_atomic_views_gname, drop_OCV_clear]{#q} SV%I.  
+  
+  Lemma know_na_view_agree ℓ p q V V' :
+    know_na_view ℓ q V -∗
+    know_na_view ℓ p V' -∗
+    ⌜ V = V' ⌝.
+  Proof.
+    apply: ghost_map_elem_agree.
+  Qed.
+
+  Global Instance know_na_view_fractional ℓ V :
+    Fractional (λ q, know_na_view ℓ q V).
+  Proof. apply _. Qed.
+
+  Global Instance know_na_view_as_fractional ℓ V q :
+    AsFractional (know_na_view ℓ q V)
+      (λ q, know_na_view ℓ q V) q.
+  Proof. apply _. Qed.
+
+  #[global] Instance know_na_view_into_nextgen ℓ q (SV: view):
+    IntoNextgen
+      (know_na_view ℓ q SV)
+      (if_rec ℓ (know_na_view ℓ q ∅)).
+  Proof.
+    rewrite /IntoNextgen /know_na_view.
+    iIntros "know !>" (OCV ?) "#OCV _".
+    iDestruct "know" as "[_ know]".
+    iApply "know"; first done.
+    rewrite elem_of_dom //.
+  Qed.
+End NAView.
+(* so that iDestruct will prioritize fractional lemma over splitting [gen_own] *)
+#[global] Opaque know_na_view.
+
+Definition new_hist t (bumper : positive → option positive) (hist : gmap time positive) :=
+  omap bumper (map_extra.drop_above t hist).
+
+Section Histories.
+  Context `{nvmHighGS}.
+  Implicit Types (q: Qp) (ℓ: loc)
+    (enc_abs_hist : gmap time positive)
+    (abs_hists : gmap loc (gmap time positive)).
+
+  Definition know_phys_hist_msg ℓ t msg : iProp Σ :=
+    auth_map_map_frag_singleton histories_rel phy_history_name ℓ t msg.
+  
+  (** The encoded version of history assertions. *)
+  Definition know_full_encoded_history_loc ℓ q enc_abs_hist : iProp Σ :=
+    full_entry bumpers_name abs_history_name ℓ (DfracOwn q) enc_abs_hist.
+
+  Definition know_frag_encoded_history_loc ℓ t e : iProp Σ :=
+    frag_entry bumpers_name abs_history_name ℓ t e.
+
+  Context `{Countable ST}.
+  Implicit Types (abs_hist : gmap time ST).
+
+  (** The decoded version of history assertions. *)
+  Definition know_full_history_loc ℓ q abs_hist : iProp Σ :=
+    full_entry bumpers_name abs_history_name ℓ (DfracOwn q) (encode <$> abs_hist).
+
+  (* In this definition we store that decoding the stored encoded histry is
+  equal to our abstract history. This is weaker than strogin the other way
+  around, namely that encoding our history is equal to the stored encoded
+  history. Storing this weaker fact makes the definition easier to show. This is
+  important for the load lemma where, when we load some state and we want to
+  return [store_lb] for the returned state. At that point we can conclude that
+  decoding the encoding gives a result but not that the encoding is an encoding
+  of some state. *)
+  Definition know_frag_history_loc `{Countable ST} ℓ t (σ : ST) : iProp Σ :=
+    ∃ eσ, ⌜ decode eσ = Some σ ⌝ ∗ frag_entry bumpers_name abs_history_name ℓ t eσ.
+
+  Global Instance know_full_history_loc_fractional ℓ (abs_hist : gmap nat ST) :
+    Fractional (λ q, know_full_history_loc ℓ q abs_hist).
+  Proof. apply _. Qed.
+
+  Global Instance know_full_history_loc_as_fractional ℓ (abs_hist : gmap nat ST) q :
+    AsFractional (know_full_history_loc ℓ q abs_hist)
+      (λ q, know_full_history_loc ℓ q abs_hist) q.
+  Proof. apply _. Qed.
+
+  (** Lemmas above history assertions. *)
+  Lemma know_full_history_loc_agree ℓ p q abs_hist1 abs_hist2 :
+    know_full_history_loc ℓ p abs_hist1 -∗
+    know_full_history_loc ℓ q abs_hist2 -∗
+    ⌜ abs_hist1 = abs_hist2 ⌝.
+  Proof.
+    iIntros "[A _]". iIntros "[B _]".
+    iDestruct (full_entry_agree with "A B") as %<-%(inj _). done.
+  Qed.
+
+  Lemma know_full_history_loc_encode ℓ q abs_hist :
+    know_full_history_loc ℓ q abs_hist ⊣⊢
+      know_full_encoded_history_loc ℓ q (encode <$> abs_hist).
+  Proof. done. Qed.
+
+  Lemma know_frag_history_loc_decode ℓ t s :
+    know_frag_encoded_history_loc ℓ t (encode s) -∗
+    know_frag_history_loc ℓ t s.
+  Proof. iIntros "H". iExists _. iFrame. rewrite decode_encode. done. Qed.
+
+  Lemma full_map_frag_singleton_agree dq ℓ t (s : ST) hists :
+    full_map bumpers_name abs_history_name dq hists -∗
+    know_frag_history_loc ℓ t s -∗
+    ⌜∃ hist enc,
+      hists !! ℓ = Some hist ∧ hist !! t = Some enc ∧ decode enc = Some s⌝.
+  Proof.
+    iIntros "H1 (% & % & H2)".
+    iDestruct (full_map_frag_entry with "H1 H2") as %(mi & EQ & hq).
+    iPureIntro. eexists _, _. split_and!; done.
+  Qed.
+
+  Lemma know_full_encoded_history_lookup q ℓ enc_abs_hist t (s : ST) :
+    know_full_encoded_history_loc ℓ q enc_abs_hist -∗
+    know_frag_history_loc ℓ t s -∗
+    ⌜∃ enc,
+        enc_abs_hist !! t = Some enc ∧ decode enc = Some s⌝.
+  Proof.
+    rewrite /know_full_encoded_history_loc.
+    iIntros "H1 (% & % & H2)".
+    iDestruct (full_entry_frag_entry with "H1 H2") as %look.
+    iPureIntro. eexists _. split_and!; done.
+  Qed.
+
+  Lemma know_full_encoded_history_lookup_big q ℓ full_enc_hist hist :
+    know_full_encoded_history_loc ℓ q full_enc_hist -∗
+    ([∗ map] t↦s ∈ hist, know_frag_history_loc ℓ t s) -∗
+    ⌜ ∃ enc_hist,
+      enc_hist ⊆ full_enc_hist ∧
+      dom hist = dom enc_hist ∧
+      omap decode enc_hist = hist ∧
+      (* The last conjunc here is "bonus" and can be removed unless users of *)
+(*        * the lemma make use of it. *)
+      map_Forall (λ k enc, ∃ s, decode enc = Some s ∧
+                                hist !! k = Some s) enc_hist ⌝.
+  Proof.
+    iIntros "F M".
+    rewrite /know_frag_history_loc.
+    iDestruct (big_sepM_exist_r with "M") as (hist_enc) "M".
+    iDestruct (full_entry_lookup_big _ _ _ _ _ hist_enc with "F [M]") as %sub.
+    { iApply big_sepM_forall.
+      iIntros (???).
+      iDestruct (big_sepM2_lookup_r with "M") as (???) "$"; first done. }
+    iExists hist_enc.
+    iSplit; first done.
+    iDestruct (big_sepM2_dom with "M") as %domeq.
+    iSplit; first done.
+    iSplit.
+    { rewrite map_eq_iff. iIntros (t).
+      rewrite lookup_omap. destruct (hist_enc !! t) eqn:look.
+      - iDestruct (big_sepM2_lookup_r with "M") as (?  look2 ?) "hih"; first done.
+        rewrite look2. done.
+      - iPureIntro. simpl. symmetry.
+        eapply map_dom_eq_lookup_None; done. }
+    iIntros (?? look).
+    iDestruct (big_sepM2_lookup_r with "M") as (???) "hih"; first done.
+    iExists x1. done.
+  Qed.
+
+  Lemma know_frag_history_singleton_agree ℓ t s1 s2 :
+    know_frag_history_loc ℓ t s1 -∗
+    know_frag_history_loc ℓ t s2 -∗
+    ⌜ s1 = s2 ⌝.
+  Proof.
+    iDestruct 1 as (enc deq) "K".
+    iDestruct 1 as (enc' deq') "K'".
+    iDestruct (frag_entry_agree with "K K'") as %<-.
+    iPureIntro. congruence.
+  Qed.
+
+  Lemma know_full_history_lookup ℓ q abs_hist t s :
+    know_full_history_loc ℓ q abs_hist -∗
+    know_frag_history_loc ℓ t s -∗
+    ⌜ abs_hist !! t = Some s ⌝.
+  Proof.
+    iIntros "A B".
+    iDestruct ("B") as (e decEq) "B".
+    iDestruct (full_entry_frag_entry with "A B") as %look.
+    apply lookup_fmap_Some in look as (s' & encEq & look).
+    assert (s = s') as <-.
+    { rewrite -encEq decode_encode in decEq. by inversion decEq. }
+    done.
+  Qed.
+
+  (** nextgen instances *)
+
+  Definition lastgen_know_frag_history_loc `{Countable ST} ℓ t (σ : ST) : iProp Σ :=
+    ∃ eσ, ⌜ decode eσ = Some σ ⌝ ∗ lastgen_frag_entry abs_history_name ℓ t eσ.
+  
+  Context `{!AbstractState ST}.
+  #[global] Instance know_frag_history_loc_into_nextgen ℓ t (σ: ST):
+    IntoNextgen
+      (know_frag_history_loc ℓ t σ)
+      (lastgen_know_frag_history_loc ℓ t σ ∗
+       ∀ OCV (bumper: ST → ST), ⌜ ℓ ∈ dom OCV ∧ t ≤ OCV !!0 ℓ ⌝ -∗
+                                crashed_at_offset OCV -∗
+                                know_bumper ℓ bumper -∗
+                                know_frag_history_loc ℓ t (bumper σ)).
+  Proof.
+    rewrite /IntoNextgen.
+    iIntros "(%eσ & %Hdecode & frag)".
+    iModIntro.
+    iDestruct "frag" as "[lastgen_frag frag]".
+    iSplitL "lastgen_frag".
+    { iExists _. by iFrame. }
+    iIntros (OCV bumper [? ?]) "OCV [% bumper]".
+    iSpecialize ("frag" with "OCV [//] bumper").
+    rewrite /drop_above_bump decide_True; last done.
+    rewrite /encode_bumper /safe_bumper Hdecode /=.
+    iExists _. iFrame.
+    iPureIntro.
+    apply decode_encode.
+  Qed.
+End Histories.
+
+(* TODO: replace this definition with [picked_in] of abstract history *)
+Section crashed_in.
+  Context `{nvmHighGS}.
+  Context `{Countable ST}.
+
+  (* [crashed_in ℓ s] means location [ℓ] crashed in (latest) abstract state [s]
+   * (before applying bumper). *)
+  Definition crashed_in_loc (ℓ: loc) (σ : ST) : iProp Σ :=
+    ∃ eσ OCV, crashed_at_offset OCV ∗ ⌜ ℓ ∈ dom OCV ⌝ ∗ ⌜ decode eσ = Some σ ⌝ ∗ lastgen_frag_entry abs_history_name ℓ (OCV !!0 ℓ) eσ.
+
+  Lemma crashed_in_loc_agree ℓ σ1 σ2:
+    crashed_in_loc ℓ σ1 -∗ crashed_in_loc ℓ σ2 -∗ ⌜ σ1 = σ2 ⌝.
+  Proof.
+    iDestruct 1 as (??) "(#OCV & _ & % & know)".
+    iDestruct 1 as (??) "(#OCV' & _ & % & know')".
+    iDestruct (crashed_at_offset_agree with "OCV OCV'") as %->.
+    iDestruct (lastgen_frag_entry_agree with "know know'") as %->.
+    by simplify_eq.
+  Qed.
+
+  Lemma crashed_in_OCV OCV ℓ σ:
+    crashed_at_offset OCV -∗ crashed_in_loc ℓ σ -∗ ⌜ ℓ ∈ dom OCV ⌝.
+  Proof.
+    iIntros "OCV".
+    iDestruct 1 as (??) "(#OCV' & % & _)".
+    by iDestruct (crashed_at_offset_agree with "OCV OCV'") as %->.
+  Qed.
+End crashed_in.
+
+Opaque crashed_in_loc.
+
+Section NextgenLemmas.
+  Context `{!nvmBaseGS Σ Ω, !nvmHighGS Σ Ω, !PerennialG Σ}.
+  Context `{AbstractState ST}.
+
+  #[global] Instance know_bumper_nextgen ℓ (bumper: ST → ST):
+    IntoNextgen
+      (know_bumper ℓ bumper)
+      (if_rec ℓ (know_bumper ℓ bumper)).
+  Proof.
+    rewrite /IntoNextgen.
+    iIntros "[%bumpValid #bumper]".
+    iPoseProof (ghost_map_elem_into_nextgen_ifrec with "bumper") as "#bumper'".
+    iModIntro.
+    iDestruct "bumper'" as "[_ ?]".
+    iModIntro.
+    iSplit; done.
+  Qed.
+
+  (* Lemma frag_history_nextgen ℓ t offset bumper (σ : ST) : *)
+  (*   ⎡ know_preorder_loc ℓ (abs_state_relation (ST := ST)) ⎤ -∗ *)
+  (*   ⎡ offset_loc ℓ offset ⎤ -∗ *)
+  (*   ⎡ know_bumper ℓ bumper ⎤ -∗ *)
+  (*   ⎡ know_frag_history_loc ℓ t σ ⎤ -∗ *)
+  (*   <NG> if_rec ℓ (∃ σC CV tC v, *)
+  (*              ⌜ CV !! ℓ = Some (MaxNat tC) ⌝ ∗ *)
+  (*              ⎡ crashed_at CV ⎤ ∗ *)
+  (*              ⎡ crashed_in ℓ σC ⎤ ∗ *)
+  (*              ⎡ know_frag_history_loc ℓ (offset + tC) (bumper σC) ⎤ ∗ *)
+  (*              ⎡ know_phys_hist_msg ℓ (offset + tC) (memory.Msg v ∅ ∅ ∅) ⎤ ∗ *)
+  (*              (⌜ t ≤ offset + tC ⌝ -∗ *)
+  (*               ⌜ σ ⊑ σC ⌝ ∗ ⎡ know_frag_history_loc ℓ t (bumper σ) ⎤)). *)
+  (* Proof. *)
+  (*   iIntros "preOrder #offset #bumper fragHist". *)
+  (*   iPoseProof (ghost_map_elem_into_nextgen_ifrec with "preOrder") as "preOrder". *)
+  (*   rewrite /know_frag_history_loc /know_frag_history_loc. *)
+  (*   iDestruct "fragHist" as (encσ Hdecodeσ) "frag_hist_entry". *)
+  (*   iPoseProof (frag_entry_local_nextgen with "frag_hist_entry [bumper]") as "frag_hist_entry". *)
+  (*   { iDestruct "bumper" as "[? $]". } *)
+  (*   iModIntro. *)
+  (*   rewrite -?if_rec_lift_if_rec. *)
+  (*   iModIntro. *)
+  (* Abort. *)
+End NextgenLemmas.
