src/high/predicates.v
@@ -1,6 +1,6 @@
 From iris.bi Require Import lib.fractional.
 From iris.base_logic.lib Require Import own.
-From iris.algebra Require Import gset gmap excl auth gmap_view.
+From iris.algebra Require Import gset gmap excl auth gmap_view stepindex_finite.
 From iris.proofmode Require Import reduction monpred ltac_tactics.
 From iris_named_props Require Import named_props.
 
@@ -15,12 +15,13 @@ From PerennialNG.base_logic.lib Require Import wsat.
 
 Section predicates.
   Context `{nvmHighGS}.
-
+  
+  #[local] Existing Instance nvmHighGS_inG.
   (* Note, there are three types for predicates.
      1/ The real/initial type which depends on some [ST]: *)
   Definition predicate ST := ST → val → dProp Σ.
   Canonical Structure predicateO ST := ST -d> val -d> dPropO Σ.
-
+  
   (* 2/ The encoded type that doesnt depend on [ST]: *)
   Definition enc_predicate := positive → val → option (dProp Σ).
   Definition enc_predicateO := positive -d> val -d> optionO (dPropO Σ).
@@ -44,15 +45,15 @@ Section predicates.
     (pred : enc_predicateO) : predO :=
       λ s v, (λ p i, monPred_at p i) <$> (pred s v).
 
-  Definition unwrapped_pred_to_ra (pred : unwrapped_predicateO) :
-    (@predicateR Σ) :=
-    to_agree ((λ a b, Next (pred a b))).
+  Definition unwrapped_pred_to_ra (pred : unwrapped_predicateO): gen_predicates.predicateO Σ :=
+    (λ a b, Next (pred a b)).
 
-  Definition pred_to_ra (pred : enc_predicateO) : (@predicateR Σ) :=
+  Definition pred_to_ra (pred : enc_predicateO) : gen_predicates.predicateO Σ :=
     unwrapped_pred_to_ra (encoded_pred_unwrap pred).
 
-  Global Instance encoded_pred_unwrap_proper :
-    ∀ n, Proper (@dist _ enc_predicateO _ n ==> @dist _ predO _ n) encoded_pred_unwrap.
+  (* [natSI] should be automatically chosen, but I'm still debugging what went wrong. *)
+  #[global] Instance encoded_pred_unwrap_proper :
+    ∀ (n: natSI), Proper (dist (A := enc_predicateO) n ==> dist (A := predO) n) encoded_pred_unwrap.
   Proof.
     intros ? p1 p2 eq.
     rewrite /encoded_pred_unwrap.
@@ -67,23 +68,48 @@ Section predicates.
     apply eq.
   Qed.
 
-  Global Instance pred_to_ra_ne :
-    ∀ n, Proper (@dist _ enc_predicateO _ n ==> dist n) pred_to_ra.
+  #[global] Instance pred_to_ra_ne :
+    ∀ (n: natSI), Proper (dist (A := enc_predicateO) n ==> dist (A := gen_predicates.predicateO Σ) n) pred_to_ra.
   Proof.
     intros ??? eq.
     rewrite /pred_to_ra.
     rewrite /pred_to_ra.
     rewrite /unwrapped_pred_to_ra.
-    apply (@to_agree_ne _ (positive -d> val -d> laterO (optionO (thread_view -d> (iPropO Σ))))).
     intros ??.
     eassert (NonExpansive Next) as ne; last apply ne; first by apply _.
     apply encoded_pred_unwrap_proper in eq.
     specialize (eq x0).
     apply eq.
   Qed.
+  
+  #[local] Instance unwrapped_pred_to_ra_contractive :
+    Contractive unwrapped_pred_to_ra.
+  Proof.
+    rewrite /pred_to_ra.
+    rewrite /unwrapped_pred_to_ra.
+    intros ??? dl.
+    intros ??.
+    destruct n. { apply: contractive_0. }
+    apply (contractive_S Next).
+    apply dist_later_S in dl.
+    apply (dl x0 x1).
+  Qed.
+
+  (* FIXME: this lemma used to be resolved by [solve_contractive] but no longer. *)
+  #[global] Instance pred_to_ra_contractive :
+    Contractive (pred_to_ra).
+  Proof.
+    rewrite /pred_to_ra.
+    intros ??? dl ??.
+    apply: unwrapped_pred_to_ra_contractive.
+    constructor.
+    intros m ?.
+    apply (dist_later_dist_lt _ m) in dl; last done.
+    rewrite dl //.
+  Qed.
 
   Definition preds_to_ra (preds : gmap loc (enc_predicate))
-    : gmapUR loc (@predicateR Σ) := pred_to_ra <$> preds.
+    : gmap loc (gen_predicates.predicateO Σ) := pred_to_ra <$> preds.
 
   Definition own_all_preds γ dq preds :=
     own_all_preds_ra γ dq (preds_to_ra preds).
@@ -111,24 +137,6 @@ Section predicates.
 
   Definition know_pers_pred `{Countable ST} := know_pred (ST := ST) pers_predicates_name.
 
-  Local Instance unwrapped_pred_to_ra_contractive :
-    Contractive unwrapped_pred_to_ra.
-  Proof.
-    rewrite /pred_to_ra.
-    rewrite /unwrapped_pred_to_ra.
-    intros ??? dl.
-    apply (@to_agree_ne _ (positive -d> val -d> laterO (optionO (thread_view -d> (iPropO Σ))))).
-    intros ??.
-    destruct n. { apply: contractive_0. }
-    apply (contractive_S Next).
-    apply dist_later_S in dl.
-    apply (dl x0 x1).
-  Qed.
-
-  Local Instance pred_to_ra_contractive :
-    Contractive (pred_to_ra).
-  Proof. solve_contractive. Qed.
-
   Global Instance encode_predicate_ne `{Countable ST} :
     NonExpansive (encode_predicate (ST := ST)).
   Proof.
@@ -145,12 +153,10 @@ Section predicates.
   Proof.
     intros ??? Hdist.
     rewrite /know_pred /know_pred_ra /named.
-    do 4 f_equiv.
-    f_contractive.
-    apply encoded_pred_unwrap_proper.
-    simpl in Hdist.
-    rewrite Hdist.
-    f_equiv.
+    rewrite /gen_ghost_map_ofe.ghost_mapO_elem.
+    do 5 f_equiv.
+    apply pred_to_ra_contractive.
+    rewrite ne_dist_later //.
   Qed.
 
   Global Instance know_full_pred_contractive `{Countable ST} ℓ :
@@ -240,92 +246,71 @@ Section predicates.
        ⌜preds !! ℓ = Some o⌝ ∗ (* Some encoded predicate exists. *)
        ▷ (o ≡ encode_predicate ϕ)).
   Proof.
-    iNamed 1. iIntros "[own_frag _]".
-    iDestruct (gen_own_valid_2 with "own_auth own_frag") as "H".
-    iDestruct (auth_both_dfrac_validI with "H") as "(_ & tmp & val)".
-    iDestruct "tmp" as (c) "#eq".
-    rewrite gmap_equivI.
-    iSpecialize ("eq" $! ℓ).
+    iIntros "auth elem".
+    iDestruct (gen_ghost_map_ofe.ghost_mapO_lookup with "[$] [$]") as "eq".
+    rewrite /preds_to_ra /pred_to_ra /unwrapped_pred_to_ra.
     rewrite lookup_fmap.
-    rewrite lookup_op.
-    rewrite lookup_singleton_eq.
-    destruct (preds !! ℓ) as [o|] eqn:eq; rewrite eq; simpl.
-    2: {
-      case (c !! ℓ); intros; iDestruct "eq" as %eq'; rewrite Some_op_opM in eq'; inversion eq'. }
+    destruct (preds !! ℓ) as [o|] eqn:eq; rewrite eq /=;
+      last (iDestruct "eq" as %eq'; inversion eq').                                                  
     iExists o.
     iSplit; first done.
-    destruct (c !! ℓ) eqn:Heq; rewrite Heq.
-    - rewrite -Some_op.
-      rewrite !option_equivI.
-      rewrite wsat.agree_equiv_inclI.
-      rewrite !discrete_fun_equivI. iIntros (state).
-      iSpecialize ("eq" $! state).
-      rewrite !discrete_fun_equivI. iIntros (v).
-      iSpecialize ("eq" $! v).
-      rewrite later_equivI_1.
-      iNext.
-      rewrite /predicate_to_unwrapped_predicate.
-      iDestruct (encoded_pred_unwrap_inj with "eq") as "eq2".
-      iRewrite "eq2".
-      done.
-    - rewrite right_id.
-      simpl.
-      rewrite !option_equivI.
-      rewrite agree_equivI.
-      rewrite !discrete_fun_equivI. iIntros (state).
-      iSpecialize ("eq" $! state).
-      rewrite !discrete_fun_equivI. iIntros (v).
-      iSpecialize ("eq" $! v).
-      rewrite later_equivI_1.
-      iNext.
-      rewrite /predicate_to_unwrapped_predicate.
-      iDestruct (encoded_pred_unwrap_inj with "eq") as "eq2".
-      done.
+    rewrite !option_equivI.
+    rewrite !discrete_fun_equivI. iIntros (state).
+    iSpecialize ("eq" $! state).
+    rewrite !discrete_fun_equivI. iIntros (v).
+    iSpecialize ("eq" $! v).
+    rewrite later_equivI_1.
+    iNext.
+    rewrite /predicate_to_unwrapped_predicate.
+    iDestruct (encoded_pred_unwrap_inj with "eq") as "eq2".
+    iRewrite "eq2".
+    done.
   Qed.
 
-  Lemma own_all_full_preds_pred `{Countable ST}
-        dq ℓ (ϕ : predicate ST) (preds : gmap loc enc_predicate) :
-    own_all_full_preds dq preds -∗
-    know_full_pred ℓ ϕ -∗
-    (∃ (o : enc_predicateO),
-       ⌜preds !! ℓ = Some o⌝ ∗ (* Some encoded predicate exists. *)
-       ▷ (o ≡ encode_predicate ϕ)).
-    Proof. apply own_all_preds_pred. Qed.
-
-  Lemma own_all_read_preds_pred `{Countable ST}
-        dq ℓ (ϕ : predicate ST) (preds : gmap loc enc_predicate) :
-    own_all_read_preds dq preds -∗
-    know_read_pred ℓ ϕ -∗
-    (∃ (o : enc_predicateO),
-       ⌜preds !! ℓ = Some o⌝ ∗ (* Some encoded predicate exists. *)
-       ▷ (o ≡ encode_predicate ϕ)).
-  Proof. apply own_all_preds_pred. Qed.
-
-  Lemma own_all_pers_preds_pred `{Countable ST}
-        dq ℓ (ϕ : predicate ST) (preds : gmap loc enc_predicate) :
-    own_all_pers_preds dq preds -∗
-    know_pers_pred ℓ ϕ -∗
-    (∃ (o : enc_predicateO),
-       ⌜preds !! ℓ = Some o⌝ ∗ (* Some encoded predicate exists. *)
-       ▷ (o ≡ encode_predicate ϕ)).
-  Proof. apply own_all_preds_pred. Qed.
-
-  Lemma predicates_frag_lookup γ predicates (ℓ : loc) pred :
-    predicates !! ℓ = Some pred →
-    gen_own γ (◯ (pred_to_ra <$> predicates) : predicatesR) -∗
-    gen_own γ (◯ {[ ℓ := pred_to_ra pred ]}).
+  Lemma own_all_preds_insert `{Countable ST} γ preds ℓ (ϕ : ST → val → dProp Σ) :
+    preds !! ℓ = None →
+    own_all_preds γ (DfracOwn 1) preds ==∗
+    own_all_preds γ (DfracOwn 1) (<[ℓ := encode_predicate ϕ]> preds) ∗
+    know_pred γ ℓ ϕ.
   Proof.
-    intros look.
-    iIntros "H". iApply (gen_own_mono with "H").
-    apply auth_frag_mono.
-    rewrite singleton_included_l.
-    eexists _.
-    rewrite lookup_fmap look.
-    naive_solver.
+    iIntros (look) "all".
+    set pred := (encode_predicate ϕ).
+    iMod (preds_insert _ _ ℓ (pred_to_ra pred) with "all") as "[all $]".
+    { rewrite /preds_to_ra lookup_fmap look //. }
+    rewrite /preds_to_ra -fmap_insert //.
   Qed.
+
+  Global Instance own_all_preds_auth_into_nextgen γ dq preds:
+    IntoNextgen
+      (own_all_preds γ dq preds)
+      (∀ OCV,
+         crashed_at_offset OCV -∗
+         own_all_preds γ dq (extra.restrict (dom OCV) preds)).
+  Proof.
+    rewrite /IntoNextgen.
+    iIntros "own !>" (OCV) "OCV".
+    iSpecialize ("own" with "OCV").
+    rewrite /own_all_preds /restrict map_filter_fmap //.
+  Qed.
+
+  Global Instance ghost_map_elem_into_nextgen `{AbstractState ST} γ k P:
+    IntoNextgen
+      (know_pred γ (ST := ST) k P)
+      (if_rec k (know_pred γ (ST := ST) k P)).
+  Proof.
+    rewrite /IntoNextgen.
+    iIntros "know_pred !>!> //".
+  Qed.
+End predicates.
+
+Section encoded_predicate.
+  Context `{AbstractState ST}.
+  Context `{nvmHighGS}.
+
+  Implicit Types (s : ST) (ϕ : ST → val → dProp Σ).
 
   (** If [pred] is the encoding of [Φ] then [pred] holding for the encoding of *)
-(*   [s] is equivalent to [ϕ] holding for [s]. *)
+  (*  [s] is equivalent to [ϕ] holding for [s]. *)
   Lemma pred_encode_Some `{Countable ST}
         ϕ (s : ST) (v : val) (pred : enc_predicateO) :
     (pred ≡ encode_predicate ϕ : iProp Σ) -∗
@@ -338,34 +323,7 @@ Section predicates.
     rewrite /encode_predicate. rewrite decode_encode /=.
     done.
   Qed.
-
-  Lemma own_all_preds_insert `{Countable ST} γ preds ℓ (ϕ : ST → val → dProp Σ) :
-    preds !! ℓ = None →
-    own_all_preds γ (DfracOwn 1) preds ==∗
-    own_all_preds γ (DfracOwn 1) (<[ℓ := encode_predicate ϕ]> preds) ∗
-    know_pred γ ℓ ϕ.
-  Proof.
-    iIntros (look). iNamed 1.
-    rewrite /know_pred.
-    rewrite comm.
-    iMod (gen_own_update with "own_auth") as "[H $]".
-    { apply auth_update_alloc.
-      apply alloc_local_update; last done.
-      rewrite /preds_to_ra. rewrite lookup_fmap. rewrite look. done. }
-    iModIntro.
-    iFrame "#".
-    rewrite /preds_to_ra.
-    rewrite fmap_insert.
-    iFrame.
-  Qed.
-End predicates.
-
-Section encoded_predicate.
-  Context `{AbstractState ST}.
-  Context `{nvmHighGS}.
-
-  Implicit Types (s : ST) (ϕ : ST → val → dProp Σ).
-
+  
   Definition encoded_predicate_holds
     (enc_pred : positive → val → optionO (dPropO Σ))
     (enc_state : positive) (v : val) i : iProp Σ :=
@@ -436,27 +394,5 @@ Section encoded_predicate.
   Proof.
     iIntros (???). iDestruct 1 as (P) "[eq P]".
     iExists P. iFrame.
-  Qed.
-
-  Global Instance own_all_preds_auth_into_nextgen γ dq preds:
-    IntoNextgen
-      (own_all_preds γ dq preds)
-      (∀ OCV,
-         crashed_at_offset OCV -∗
-         own_all_preds γ dq (extra.restrict (dom OCV) preds)).
-  Proof.
-    rewrite /IntoNextgen.
-    iIntros "own !>" (OCV) "OCV".
-    iSpecialize ("own" with "OCV").
-    rewrite /own_all_preds /restrict map_filter_fmap //.
-  Qed.
-
-  Global Instance ghost_map_elem_into_nextgen γ k P:
-    IntoNextgen
-      (know_pred γ (ST := ST) k P)
-      (if_rec k (know_pred γ (ST := ST) k P)).
-  Proof.
-    rewrite /IntoNextgen.
-    iIntros "know_pred !>!> //".
   Qed.
 End encoded_predicate.
