src/high/lib/bumpers.v
@@ -1,0 +1,34 @@
+From stdpp Require Import countable ssreflect.
+From self Require Export options.
+
+(* Pure facts about bumpers *)
+Section bumpers.
+  Context `{Countable ST}.
+  
+  Definition encode_bumper (bumper : ST → ST) :=
+    λ e, encode <$> (bumper <$> decode e).
+
+  Lemma encode_bumper_Some_decode (bumper : ST → ST) (x x' : positive) :
+    encode_bumper bumper x = Some x' →
+    ∃ (s : ST), decode x = Some s ∧ encode (bumper s) = x'.
+  Proof.
+    rewrite /encode_bumper => eq.
+    destruct (decode x) as [s|].
+    - exists s. inversion eq. done.
+    - inversion eq.
+  Qed.
+
+  Lemma encode_bumper_encode (bumper : ST → ST) (s : ST) :
+    encode_bumper bumper (encode s) = Some (encode (bumper s)).
+  Proof. rewrite /encode_bumper. rewrite decode_encode. done. Qed.
+
+  (* An encoded bumper returns some encoded value then that encoded value will
+  also result in some other encoded bumper again. This represents that encoded
+  bumpers take "valid" encodings to "valid" encodings. *)
+  Lemma encode_bumper_bump_to_valid bumper e e' :
+    encode_bumper bumper e = Some e' → is_Some (encode_bumper bumper e').
+  Proof.
+    intros (s' & ? & encodeEq)%encode_bumper_Some_decode.
+    rewrite <- encodeEq. rewrite encode_bumper_encode. done.
+  Qed.
+End bumpers.
