src/high/resources/gen_alocs.v
@@ -8,18 +8,18 @@ From iris_named_props Require Import named_props.
 From self Require Import extra map_extra.
 From self.nextgen Require Import hvec nextgen_promises.
 From self.algebra Require Import view.
-From self.base Require Import generational_resources.
+From self.base Require Import generational_resources if_rec.
 
 From self.lang Require Import lang.
+
+Definition gen_alocsR: cmra := authR (gsetUR loc).
+Notation gen_alocsR_inG Σ Ω := (genInDepsG Σ Ω (gen_alocsR) [#crashed_atR]).
 
 (* similar to [gen_ghost_map], the transformer depends on the [crashed_at] resrouce.
  * since there is only one transformer we need, I'm not generalizing the definitions.
  * I hope it will not cause troubles later... *)
 Section gen_alocs.
   Implicit Type (OCV: view) (ℓs: gset loc).
-
-  Definition gen_alocsR: cmra := authR (gsetUR loc).
-  Notation gen_alocsR_inG Σ Ω := (genInDepsG Σ Ω (gen_alocsR) [#crashed_atR]).
 
   Definition drop_OCV_locs OCV ℓs :=
     ℓs ∩ dom OCV.
@@ -30,9 +30,21 @@ Section gen_alocs.
         tC = crashed_at_trans OCV ∧
         t = fmap_auth $ drop_OCV_locs OCV.
 
-  #[local] Existing Instance nvmBaseGS_crashed_at_inG.
-  #[local] Existing Instance crashed_atGpreS_crashed_at.
-
+  #[local] Instance drop_OCV_locs_cmra_morphism OCV:
+    CmraMorphism (fmap_auth (drop_OCV_locs OCV)).
+  Proof.
+    apply: fmap_auth_gentrans.
+    split; try done.
+    - intros n locs1 locs2.
+      rewrite -?discrete_iff.
+      fold_leibniz.
+      congruence.
+    - intros.
+      fold_leibniz.
+      rewrite /drop_OCV_locs gset_op.
+      set_solver.
+  Qed.
+  
   Context `{!nvmBaseGS Σ Ω} `{!gen_alocsR_inG Σ Ω}.
 
   Definition gen_alocs_auth γ ℓs: iProp Σ :=
@@ -45,6 +57,70 @@ Section gen_alocs.
     "#rely" ∷ rely γ [#crashed_at_name] gen_alocs_rel (λ _, true) ∗
     "#crashed" ∷ ∃ OCV, crashed_at_offset OCV.
 
+  Lemma gen_alocs_update {γ} locs ℓ :
+    gen_alocs_auth γ locs ==∗ gen_alocs_auth γ (locs ∪ {[ ℓ ]}) ∗ gen_alocs_frag γ {[ ℓ ]}.
+  Proof.
+    iNamed 1.
+    iDestruct (@gen_own_update with "own_auth") as ">[auth frag]".
+    { apply auth_update_alloc. apply gset_local_update.
+      apply (union_subseteq_r {[ ℓ ]}). }
+    rewrite /gen_alocs_auth /gen_alocs_frag.
+    iFrame "#".
+    iEval (rewrite -gset_op) in "frag". iDestruct "frag" as "[$ _]".
+    rewrite (comm (∪)).
+    iFrame.
+    done.
+  Qed.
+
+  Lemma gen_alocs_agree {γ} locs1 locs2 :
+    gen_alocs_auth γ locs1 -∗ gen_alocs_frag γ locs2 -∗ ⌜ locs2 ⊆ locs1 ⌝.
+  Proof.
+    iNamed 1.
+    iDestruct 1 as "[own_frag _]".
+    iDestruct (gen_own_valid_2 with "own_auth [$]") as %[H%gset_included _]%auth_both_valid_discrete.
+    done.
+  Qed.
+
+  Lemma gen_alocs_alloc locs OCV OPV:
+    crashed_at_offset OCV -∗
+    rely_self crashed_at_name (crashed_at_pred OPV) ==∗
+    ∃ γ, gen_alocs_auth γ locs ∗ gen_alocs_frag γ locs.
+  Proof.
+    iIntros "#OCV #rely".
+    iMod (own_gen_alloc
+                  (DS := [#crashed_atR])
+                  (● locs ⋅ ◯ locs)
+                  [#crashed_at_name]
+                  [##_] with "[]") as (γ) "[[$ $] tok]".
+    { apply auth_both_valid_2; done. }
+    { iIntros (i').
+      dependent elimination i' as [0%fin].
+      iAssumption. }
+    iFrame "#".
+    iMod (token_strengthen_promise
+            (DS := [#crashed_atR])
+            _ [#_] [##_] _ (gen_alocs_rel) _ True_pred
+           with "[] tok") as "tok".
+    { intros ???. unfold True_rel. rewrite huncurry_curry. done. }
+    { done. }
+    { intros ts. dependent elimination ts. done. }
+    2: {
+      iIntros (i').
+      dependent elimination i' as [0%fin].
+      iApply "rely". }
+    (* TODO: this subgoal requires me to prove that for any transformer picked for
+     * [crashed_atR], there exists a transformer for the map that satisfy [R].
+     * this can only be proven given specific [R]. I should move this lemma around. *)
+    { intros ts crashedPred.
+      dependent elimination ts as [hcons tC hnil].
+      destruct crashedPred as ((OCV2 & ? & ->) & _).
+      exists (fmap_auth $ drop_OCV_locs OCV2).
+      split; first apply _.
+      simpl.
+      exists OCV2. done. }
+    by iDestruct (token_to_rely with "tok") as "#$".
+  Qed.
+    
   #[global] Instance gen_alocs_auth_into_nextgen {γ} ℓs:
     IntoNextgen
       (gen_alocs_auth γ ℓs)
@@ -75,39 +151,26 @@ Section gen_alocs.
   #[global] Instance gen_alocs_frag_into_nextgen {γ} ℓs:
     IntoNextgen
       (gen_alocs_frag γ ℓs)
-      (∃ OCV,
-          gen_alocs_frag γ (ℓs ∩ dom OCV) ∗
-          picked_in crashed_at_name (crashed_at_trans OCV)).
+      (∀ OCV, crashed_at_offset OCV -∗ gen_alocs_frag γ (ℓs ∩ dom OCV)).
   Proof using Type.
     rewrite /IntoNextgen.
     iNamed 1.
-    iDestruct "crashed" as (OCV) "crashed".
     iModIntro.
-    iDestruct ("own_frag") as (t) "[#picked own_frag]".
-    iDestruct "rely" as "(rely & (%t' & %tC & (%R & _) & picked' & pickedC))".
-    iPickedInAgree "picked picked'".
-    destruct R as (OCV' & -> & ->).
-    iExists OCV'.
-    rewrite fmap_auth_frag /drop_OCV_locs.
-    iDestruct "crashed" as (??) "[pickedC' #crashed_at]".
+    iDestruct "crashed" as (OV OCV' tC) "[pickedC crashed]".
+    iDestruct "rely" as "[rely (%tH & %tC' & [% _] & pickedH & pickedC')]".
+    iDestruct "own_frag" as (tH') "[#pickedH' own_frag]".
     iPickedInAgree "pickedC pickedC'".
+    iPickedInAgree "pickedH pickedH'".
+    destruct H as (OCV'' & -> & ->).
+    iIntros (?) "offset".
+    simpl.
+    iAssert ⌜ OCV = OCV'' ⌝%I as %<-.
+    { iNamed "offset".
+      iDestruct (crashed_at_both_agree with "offset crashed") as %[-> ->].
+      done. }
+    rewrite fmap_auth_frag /drop_OCV_locs.
     iFrame "∗#".
-    Qed.
-
-  Lemma gen_alocs_update {γ} locs ℓ :
-    gen_alocs_auth γ locs ==∗ gen_alocs_auth γ (locs ∪ {[ ℓ ]}) ∗ gen_alocs_frag γ {[ ℓ ]}.
-  Proof.
-    iNamed 1.
-    iDestruct (@gen_own_update with "own_auth") as ">[auth frag]".
-    { apply auth_update_alloc. apply gset_local_update.
-      apply (union_subseteq_r {[ ℓ ]}). }
-    rewrite /gen_alocs_auth /gen_alocs_frag.
-    iFrame "#".
-    iEval (rewrite -gset_op) in "frag". iDestruct "frag" as "[$ _]".
-    rewrite (comm (∪)).
-    iFrame.
-    done.
   Qed.
 End gen_alocs.
 
-Notation gen_alocsR_inG Σ Ω := (genInDepsG Σ Ω (gen_alocsR) [#crashed_atR]).
+Opaque gen_alocs_auth gen_alocs_frag.
